bindinginst

coq/JsCorrectness.v
@@ -1927,6 +1927,55 @@ Admitted. (* faster *)
 
 
 
+
+Lemma creating_function_object_proto_correct : forall runs S C l o,
+  runs_type_correct runs ->
+  creating_function_object_proto runs S C l = o ->
+  red_expr S C (spec_creating_function_object_proto l) o.
+Proof.
+  introv IH HR. unfolds in HR.
+  run red_spec_creating_function_object_proto 
+    using run_construct_prealloc_correct.
+  let_simpl. run red_spec_creating_function_object_proto_1.
+  let_simpl. applys* red_spec_creating_function_object_proto_2. run_hyp*.
+Admitted. (* faster *)
+
+Lemma creating_function_object_correct : forall runs S C names bd X str o,
+  runs_type_correct runs ->
+  creating_function_object runs S C names bd X str = o ->
+  red_expr S C (spec_creating_function_object names bd X str) o.
+Proof.
+  introv IH HR. unfolds in HR.  
+  let_simpl. let_simpl. let_simpl. let_name. destruct p as [l S1].
+  let_simpl. run* red_spec_creating_function_object. rewrite* EQp. 
+    skip. (*one bug*)
+  run red_spec_creating_function_object_1 
+    using creating_function_object_proto_correct.
+  case_if; destruct str; tryfalse.
+    run_inv. applys* red_spec_creating_function_object_2_not_strict.
+    let_simpl. let_simpl. 
+     run* red_spec_creating_function_object_2_strict. clear EQp.
+     run* red_spec_creating_function_object_3.
+     applys* red_spec_creating_function_object_4.
+Admitted. (* faster*)
+
+
+
+Lemma env_record_has_binding_correct : forall runs S C L x o,
+  runs_type_correct runs ->
+  env_record_has_binding runs S C L x = o ->
+  red_expr S C (spec_env_record_has_binding L x) o.
+Proof.
+  introv IH HR. unfolds in HR. run_simpl. 
+  forwards B: @pick_option_correct (rm E).
+  applys~ red_spec_env_record_has_binding B. destruct x0; run_inv.
+   apply~ red_spec_env_record_has_binding_1_decl. 
+    rewrite decide_def; auto.
+   apply~ red_spec_env_record_has_binding_1_object.
+    apply* object_has_prop_correct.
+Qed.
+
+
 Fixpoint binding_inst_function_decls runs S C L (fds : list funcdecl) str bconfig {struct fds} : result_void :=
   match fds with
   | nil => res_void S
@@ -1962,75 +2011,148 @@ Fixpoint binding_inst_function_decls runs S C L (fds : list funcdecl) str bconfi
             if_void (env_record_create_mutable_binding runs S2 C L fname (Some bconfig)) follow))
   end.
 
+Axiom red_spec_binding_inst_function_decls_nil : forall L S C args str bconfig, (* Step 5b *)
+      red_expr S C (spec_binding_inst_function_decls args L nil str bconfig) (out_void S)
+.
+
+Axiom red_spec_binding_inst_function_decls_cons : forall str_fd S C L args fd fds str bconfig o1 o, (* Step 5b *)
+      str_fd = funcbody_is_strict (funcdecl_body fd) ->
+      red_expr S C (spec_creating_function_object (funcdecl_parameters fd) (funcdecl_body fd) (execution_ctx_variable_env C) str_fd) o1 ->
+      red_expr S C (spec_binding_inst_function_decls_1 args L fd fds str bconfig o1) o ->
+      red_expr S C (spec_binding_inst_function_decls args L (fd::fds) str bconfig) o
+.
+
 
 (* TODO: remove args from the pretty big step rules *)
+Axiom 
+ red_spec_binding_inst_function_decls_4 : forall S0 S C args L fd fds str fo bconfig rv o, (* Step 5e iii *)
+      red_expr S C (spec_binding_inst_function_decls_5 args L fd fds str fo bconfig) o ->
+      red_expr S0 C (spec_binding_inst_function_decls_4 args L fd fds str fo bconfig (out_ter S rv)) o
+.
 
 Lemma binding_inst_function_decls_correct : forall runs S C args L fds str bconfig o,
   runs_type_correct runs ->
   binding_inst_function_decls runs S C L fds str bconfig = o ->
   red_expr S C (spec_binding_inst_function_decls args L fds str bconfig) o.
+Proof.
+  introv IH HR. gen S o. induction fds; introv HR.
+  simpls. run_inv. applys* red_spec_binding_inst_function_decls_nil.
+  simpls. let_name. let_name. let_name. let_name.
+  run (@red_spec_binding_inst_function_decls_cons str_fd)
+    using creating_function_object_correct. subst*. subst*. clear R1.
+  let_name as M. rename a into fd. rename l into fo.
+  asserts M_correct: (forall S o,
+      M S = o ->
+      red_expr S C (spec_binding_inst_function_decls_5 args L fd fds str fo bconfig) o).
+    clears HR S o. introv HR. subst M.
+    subst fname. run red_spec_binding_inst_function_decls_5
+      using env_record_set_mutable_binding_correct.
+    applys* red_spec_binding_inst_function_decls_6. 
+    clear EQM.  
+  subst fname. run red_spec_binding_inst_function_decls_1
+    using env_record_has_binding_correct.
+  case_if; subst.
+    case_if; try subst L.
+Axiom
+red_spec_binding_inst_function_decls_2_true_global : forall S0 S C args fd fds str fo bconfig y1 o, (* Step 5e ii *)
+      red_spec S C (spec_object_get_prop prealloc_global (funcdecl_name fd)) y1 ->
+      red_expr S C (spec_binding_inst_function_decls_3 args fd fds str fo bconfig y1) o ->
+      red_expr S0 C (spec_binding_inst_function_decls_2 args env_loc_global_env_record fd fds str fo bconfig (out_ter S true)) o
+.
+Axiom
+red_spec_binding_inst_function_decls_3_true : forall S0 S C args fd fds str fo bconfig A Anew o1 o, (* Step 5e iii *)
+      attributes_configurable A = true ->
+      Anew = attributes_data_intro undef true true bconfig -> 
+      red_expr S C (spec_object_define_own_prop prealloc_global (funcdecl_name fd) Anew true) o1 ->
+      red_expr S C (spec_binding_inst_function_decls_4 args env_loc_global_env_record fd fds str fo bconfig o1) o ->
+      red_expr S0 C (spec_binding_inst_function_decls_3 args fd fds str fo bconfig (ret S (full_descriptor_some A))) o
+.      
+      run red_spec_binding_inst_function_decls_2_true_global
+        using run_object_get_prop_correct.
+       destruct a; tryfalse. case_if.
+         let_name. run* red_spec_binding_inst_function_decls_3_true.
+          applys* red_spec_binding_inst_function_decls_4. 
+         case_if. 
+(*
+           destruct a.
+red_spec_binding_inst_function_decls_3_false
+           run red_spec_binding_inst_function_decls_3_false_type_error.
+
+    run red_spec_binding_inst_function_decls_2_false
+      using env_record_create_mutable_binding_correct.
+     applys* red_spec_binding_inst_function_decls_4. 
+*)
 Admitted.
 
-Fixpoint binding_inst_var_decls runs S C L (vds : list string) bconfig str : result_void :=
-  match vds with
-  | nil => res_void S
-  | vd :: vds' =>
-    Let bivd := fun S => binding_inst_var_decls runs S C L vds' bconfig str in
-    if_bool (env_record_has_binding runs S C L vd) (fun S1 has =>
-      if has then
-        bivd S
-      else
-        if_void (env_record_create_set_mutable_binding runs S1 C L vd (Some bconfig) undef str) bivd)
-  end.
+(* TODO: change rules 
+
+  | red_spec_binding_inst_function_decls_3_false_type_error : forall S0 S C args fd fds str fo A bconfig o1 L o, (* Step 5e iv *)
+      attributes_configurable A = false -> 
+      descriptor_is_accessor A \/ (attributes_writable A = false \/ attributes_enumerable A = false) ->
+      red_expr S C (spec_error native_error_type) o ->
+      red_expr S0 C (spec_binding_inst_function_decls_3 args fd fds str fo bconfig (ret S (full_descriptor_some A))) o
+
+  | red_spec_binding_inst_function_decls_3_false : forall S0 S C args fd fds str fo Ad bconfig o1 L o, (* Step 5e iv else *)
+      attributes_data_configurable Ad = false -> 
+      attributes_data_writable Ad = true /\ attributes_data_enumerable Ad = true ->
+      red_expr S C (spec_binding_inst_function_decls_5 args env_loc_global_env_record fd fds str fo bconfig) o ->
+      red_expr S0 C (spec_binding_inst_function_decls_3 args fd fds str fo bconfig (dret S (attributes_data_of Ad))) o
+
+  | red_spec_binding_inst_function_decls_2_true : forall o1 L S0 S C args fd fds str fo bconfig o, (* Step 5e *)
+      L <> env_loc_global_env_record ->
+      red_expr S C (spec_binding_inst_function_decls_5 args L fd fds str fo bconfig) o ->
+      red_expr S0 C (spec_binding_inst_function_decls_2 args L fd fds str fo bconfig (out_ter S true)) o
+
+*)
 
 Lemma binding_inst_var_decls_correct : forall runs S C L vds bconfig str o,
   runs_type_correct runs ->
   binding_inst_var_decls runs S C L vds bconfig str = o ->
   red_expr S C (spec_binding_inst_var_decls L vds bconfig str) o.
+Proof.
+  introv IH HR. gen S o. induction vds; introv HR.
+  simpls. run_inv. applys* red_spec_binding_inst_var_decls_nil.
+  simpls. let_simpl.
+  run red_spec_binding_inst_var_decls_cons
+    using env_record_has_binding_correct.
+  case_if; subst.
+    applys* red_spec_binding_inst_var_decls_1_true.
+    run red_spec_binding_inst_var_decls_1_false
+      using env_record_create_set_mutable_binding_correct.
+     applys* red_spec_binding_inst_var_decls_2.
 Admitted.
-
-
-Fixpoint binding_inst_formal_params runs S C L (args : list value) (names : list string) str {struct names} : result_void :=
-  match names with
-  | nil => res_void S
-  | argname :: names' =>
-    Let v := hd undef args in
-    if_bool (env_record_has_binding runs S C L argname) (fun S1 hb =>
-      Let follow := fun S' =>
-        if_void (env_record_set_mutable_binding runs S' C L argname v str) (fun S'' =>
-          binding_inst_formal_params runs S'' C L (tl args) names' str)
-        in
-      if hb then
-        follow S1
-      else
-        if_void (env_record_create_mutable_binding runs S1 C L argname None) follow)
-  end.
-
+  
 Lemma binding_inst_formal_params_correct : forall runs S C L args names str o,
   runs_type_correct runs ->
   binding_inst_formal_params runs S C L args names str = o ->
   red_expr S C (spec_binding_inst_formal_params args L names str) o.
-Admitted.
-
-
-Lemma env_record_has_binding_correct : forall runs S C L x o,
-  runs_type_correct runs ->
-  env_record_has_binding runs S C L x = o ->
-  red_expr S C (spec_env_record_has_binding L x) o.
 Proof.
-  introv IH HR. unfolds in HR. run_simpl. 
-  forwards B: @pick_option_correct (rm E).
-  applys~ red_spec_env_record_has_binding B. destruct x0; run_inv.
-   apply~ red_spec_env_record_has_binding_1_decl. 
-    rewrite decide_def; auto.
-   apply~ red_spec_env_record_has_binding_1_object.
-    apply* object_has_prop_correct.
-Qed.
+  introv IH HR. gen S args o. induction names; introv HR.
+  simpls. run_inv. applys* red_spec_binding_inst_formal_params_empty.
+  simpls.
+  let_name. let_name.
+  run (@red_spec_binding_inst_formal_params_non_empty v args')
+    using env_record_has_binding_correct.
+    subst v args'. destruct* args.
+  let_name as M. asserts M_correct: (forall S o,
+      M S = o ->
+      red_expr S C (spec_binding_inst_formal_params_3 args' L a names str v) o).
+    clears HR S o. introv HR. subst M.
+    run red_spec_binding_inst_formal_params_3
+      using env_record_set_mutable_binding_correct.
+    applys* red_spec_binding_inst_formal_params_4. 
+    clear EQM.
+  case_if; subst.
+    applys* red_spec_binding_inst_formal_params_1_declared.
+     run red_spec_binding_inst_formal_params_1_not_declared
+       using env_record_create_mutable_binding_correct.
+    applys* red_spec_binding_inst_formal_params_2. 
+Admitted. (* faster *)
 
 Lemma binding_inst_arg_obj_correct : forall runs S C lf p xs args L o,
   binding_inst_arg_obj runs S C lf p xs args L = o ->
   red_expr S C (spec_binding_inst_arg_obj lf p xs args L) o.
-Admitted. (* argument object *)
+Admitted. (* Argument object: not done for the moment *)
 
 
 Lemma execution_ctx_binding_inst_correct : forall runs S C ct funco (p:prog) args o,
@@ -2225,37 +2347,8 @@ Admitted. (*faster*)
 
 
 
-Lemma creating_function_object_proto_correct : forall runs S C l o,
-  runs_type_correct runs ->
-  creating_function_object_proto runs S C l = o ->
-  red_expr S C (spec_creating_function_object_proto l) o.
-Proof.
-  introv IH HR. unfolds in HR.
-  run red_spec_creating_function_object_proto 
-    using run_construct_prealloc_correct.
-  let_simpl. run red_spec_creating_function_object_proto_1.
-  let_simpl. applys* red_spec_creating_function_object_proto_2. run_hyp*.
-Admitted. (* faster *)
 
 
-Lemma creating_function_object_correct : forall runs S C names bd X str o,
-  runs_type_correct runs ->
-  creating_function_object runs S C names bd X str = o ->
-  red_expr S C (spec_creating_function_object names bd X str) o.
-Proof.
-  introv IH HR. unfolds in HR.  
-  let_simpl. let_simpl. let_simpl. let_name. destruct p as [l S1].
-  let_simpl. run* red_spec_creating_function_object. rewrite* EQp. 
-    skip. (*one bug*)
-  run red_spec_creating_function_object_1 
-    using creating_function_object_proto_correct.
-  case_if; destruct str; tryfalse.
-    run_inv. applys* red_spec_creating_function_object_2_not_strict.
-    let_simpl. let_simpl. 
-     run* red_spec_creating_function_object_2_strict. clear EQp.
-     run* red_spec_creating_function_object_3.
-     applys* red_spec_creating_function_object_4.
-Admitted. (* faster*)
 
 
 
